library/init/data/list/basic.lean
@@ -16,7 +16,7 @@ variables {α : Type u} {β : Type v} {γ : Type w}
 
 namespace List
 
-protected def hasDecEq [DecidableEq α] : ∀ a b : List α, Decidable (a = b)
+protected def hasDecEq [DecidableEq α] : ∀ (a b : List α), Decidable (a = b)
 | []      []      := isTrue rfl
 | (a::as) []      := isFalse (fun h => List.noConfusion h)
 | []      (b::bs) := isFalse (fun h => List.noConfusion h)
@@ -325,7 +325,7 @@ inductive Less [HasLess α] : List α → List α → Prop
 instance [HasLess α] : HasLess (List α) :=
 ⟨List.Less⟩
 
-instance hasDecidableLt [HasLess α] [h : DecidableRel HasLess.Less] : ∀ l₁ l₂ : List α, Decidable (l₁ < l₂)
+instance hasDecidableLt [HasLess α] [h : DecidableRel HasLess.Less] : ∀ (l₁ l₂ : List α), Decidable (l₁ < l₂)
 | []      []      := isFalse (fun h => match h with end)
 | []      (b::bs) := isTrue (Less.nil _ _)
 | (a::as) []      := isFalse (fun h => match h with end)
@@ -350,7 +350,7 @@ instance hasDecidableLt [HasLess α] [h : DecidableRel HasLess.Less] : ∀ l₁ 
 instance [HasLess α] : HasLessEq (List α) :=
 ⟨List.LessEq⟩
 
-instance hasDecidableLe [HasLess α] [h : DecidableRel (HasLess.Less : α → α → Prop)] : ∀ l₁ l₂ : List α, Decidable (l₁ ≤ l₂) :=
+instance hasDecidableLe [HasLess α] [h : DecidableRel (HasLess.Less : α → α → Prop)] : ∀ (l₁ l₂ : List α), Decidable (l₁ ≤ l₂) :=
 fun a b => Not.Decidable
 
 /--  `isPrefixOf l₁ l₂` returns `true` Iff `l₁` is a prefix of `l₂`. -/
